Alternate shapes of handlers...

src/coq/Handlers/Global.v
@@ -49,10 +49,12 @@ Section Globals.
 
   Open Scope monad_scope.
   Section PARAMS.
-    Variable (E F G : Type -> Type).
-    Context `{FailureE -< E +' F +' G}.
+    Variable (E F G H : Type -> Type).
+    Context `{FailureE -< G}.
     Notation Effin := (E +' F +' (GlobalE k v) +' G).
     Notation Effout := (E +' F +' G).
+    Notation Effin' := (E +' F +' H +' (GlobalE k v) +' G).
+    Notation Effout' := (E +' F +' H +' G).
 
     Definition E_trigger {M} : forall R, E R -> (stateT M (itree Effout) R) :=
       fun R e m => r <- trigger e ;; ret (m, r).
@@ -63,8 +65,23 @@ Section Globals.
     Definition G_trigger {M} : forall R , G R -> (stateT M (itree Effout) R) :=
       fun R e m => r <- trigger e ;; ret (m, r).
 
+    Definition E_trigger' {M} : forall R, E R -> (stateT M (itree Effout') R) :=
+      fun R e m => r <- trigger e ;; ret (m, r).
+
+    Definition F_trigger' {M} : forall R, F R -> (stateT M (itree Effout') R) :=
+      fun R e m => r <- trigger e ;; ret (m, r).
+
+    Definition H_trigger' {M} : forall R, H R -> (stateT M (itree Effout') R) :=
+      fun R e m => r <- trigger e ;; ret (m, r).
+
+    Definition G_trigger' {M} : forall R , G R -> (stateT M (itree Effout') R) :=
+      fun R e m => r <- trigger e ;; ret (m, r).
+
     Definition interp_global  : itree Effin ~> stateT map (itree Effout) :=
       interp_state (case_ E_trigger (case_ F_trigger (case_ handle_global G_trigger))).
+
+    Definition interp_global'  : itree Effin' ~> stateT map (itree Effout') :=
+      interp_state (case_ E_trigger' (case_ F_trigger' (case_ H_trigger' (case_ handle_global G_trigger')))).
 
     Lemma interp_global_bind :
       forall (R S : Type) (t : itree Effin R) (k : R -> itree Effin S) s,
@@ -82,6 +99,26 @@ Section Globals.
     Lemma interp_global_ret :
       forall (R : Type) g (x: R),
         runState (interp_global (Ret x: itree Effin R)) g ≅ Ret (g,x).
+    Proof.
+      intros; apply interp_state_ret.
+    Qed.
+
+    Lemma interp_global'_bind :
+      forall (R S : Type) (t : itree Effin' R) (k : R -> itree Effin' S) s,
+        runState (interp_global' (ITree.bind t k)) s ≅
+         ITree.bind (runState (interp_global' t) s) (fun '(s',r) => runState (interp_global' (k r)) s').
+    Proof.
+      intros.
+      unfold interp_global.
+      setoid_rewrite interp_state_bind.
+      apply eq_itree_clo_bind with (UU := Logic.eq).
+      reflexivity.
+      intros [] [] EQ; inv EQ; reflexivity.
+    Qed.
+
+    Lemma interp_global'_ret :
+      forall (R : Type) g (x: R),
+        runState (interp_global' (Ret x: itree Effin' R)) g ≅ Ret (g,x).
     Proof.
       intros; apply interp_state_ret.
     Qed.
