src/coq/Handlers/Memory.v
@@ -718,10 +718,12 @@ Admitted.
 
    *)
   Section PARAMS.
-    Variable (E F : Type -> Type).
+    Variable (E F G : Type -> Type).
     Context `{FailureE -< F} `{UBE -< F}.
     Notation Effin := (E +' IntrinsicE +' MemoryE +' F).
     Notation Effout := (E +' F).
+    Notation Effin' := (E +' G +' IntrinsicE +' MemoryE +' F).
+    Notation Effout' := (E +' G +' F).
 
     Definition E_trigger {M} : forall R, E R -> (stateT M (itree Effout) R) :=
       fun R e m => r <- trigger e ;; ret (m, r).
@@ -729,9 +731,22 @@ Admitted.
     Definition F_trigger {M} : forall R, F R -> (stateT M (itree Effout) R) :=
       fun R e m => r <- trigger e ;; ret (m, r).
 
+    Definition E_trigger' {M} : forall R, E R -> (stateT M (itree Effout') R) :=
+      fun R e m => r <- trigger e ;; ret (m, r).
+
+    Definition F_trigger' {M} : forall R, F R -> (stateT M (itree Effout') R) :=
+      fun R e m => r <- trigger e ;; ret (m, r).
+
+    Definition G_trigger' {M} : forall R, G R -> (stateT M (itree Effout') R) :=
+      fun R e m => r <- trigger e ;; ret (m, r).
+
     Definition interp_memory :
       itree Effin ~> stateT memory_stack (itree Effout) :=
       interp_state (case_ E_trigger (case_ handle_intrinsic (case_ handle_memory F_trigger))).
+
+    Definition interp_memory' :
+      itree Effin' ~> stateT memory_stack (itree Effout') :=
+      interp_state (case_ E_trigger' (case_ G_trigger' (case_ handle_intrinsic (case_ handle_memory F_trigger')))).
 
     Lemma interp_memory_bind :
       forall (R S : Type) (t : itree Effin R) (k : R -> itree Effin S) m,
@@ -749,6 +764,26 @@ Admitted.
     Lemma interp_memory_ret :
       forall (R : Type) g (x: R),
         runState (interp_memory (Ret x: itree Effin R)) g ≅ Ret (g,x).
+    Proof.
+      intros; apply interp_state_ret.
+    Qed.
+
+    Lemma interp_memory'_bind :
+      forall (R S : Type) (t : itree Effin' R) (k : R -> itree Effin' S) m,
+        runState (interp_memory' (ITree.bind t k)) m ≅
+                 ITree.bind (runState (interp_memory' t) m) (fun '(m',r) => runState (interp_memory' (k r)) m').
+    Proof.
+      intros.
+      unfold interp_memory.
+      setoid_rewrite interp_state_bind.
+      apply eq_itree_clo_bind with (UU := Logic.eq).
+      reflexivity.
+      intros [] [] EQ; inv EQ; reflexivity.
+    Qed.
+
+    Lemma interp_memory'_ret :
+      forall (R : Type) g (x: R),
+        runState (interp_memory' (Ret x: itree Effin' R)) g ≅ Ret (g,x).
     Proof.
       intros; apply interp_state_ret.
     Qed.
